small steps towards improving subsume_list

examples/mutable_map.c
@@ -140,6 +140,7 @@ size_t fsm_probe(struct fixed_size_map *m, size_t key) {
 [[rc::ensures("{count - 1 <= count2}", "{length items <= length items2}")]]
  [[rc::lemmas("fsm_invariant_insert")]]
  [[rc::tactics("all: try by erewrite length_filter_insert => //; solve_goal.")]]
+ [[rc::tactics("all: try by eexists _; solve_goal.")]]
 void *fsm_insert(struct fixed_size_map *m, size_t key, void *value) {
     fsm_realloc_if_necessary(m);
     size_t slot_idx = fsm_probe(m, key);
@@ -165,6 +166,7 @@ void *fsm_insert(struct fixed_size_map *m, size_t key, void *value) {
 [[rc::ensures("own m : {alter (λ _, place p) key mp, items2, count} @ fixed_size_map")]]
  [[rc::lemmas("fsm_invariant_alter")]]
  [[rc::tactics("all: try by erewrite length_filter_insert => //; solve_goal.")]]
+ [[rc::tactics("all: try by eexists _; solve_goal.")]]
  [[rc::tactics("all: try by apply inhabitant.")]]
 void *fsm_get(struct fixed_size_map *m, size_t key) {
     size_t slot_idx = fsm_probe(m, key);
@@ -184,6 +186,7 @@ void *fsm_get(struct fixed_size_map *m, size_t key) {
 [[rc::ensures("own m : {delete key mp, items2, count} @ fixed_size_map")]]
  [[rc::lemmas("fsm_invariant_delete")]]
  [[rc::tactics("all: try by erewrite length_filter_insert => //; solve_goal.")]]
+ [[rc::tactics("all: try by eexists _; solve_goal.")]]
 void *fsm_remove(struct fixed_size_map *m, size_t key) {
     void* removed;
     size_t slot_idx = fsm_probe(m, key);
