tutorial/proofs/t05_main/generated_proof_main2.v
@@ -13,7 +13,7 @@ Section proof_main2.
   (* Typing proof for [main2]. *)
   Lemma type_main2 (global_initialized global_latch_wait global_test : loc) :
     global_locs !! "initialized" = Some global_initialized →
-    global_initialized_types !! "initialized" = Some (GT () (λ '(), (latch (alloc_initialized)) : type)) →
+    global_initialized_types !! "initialized" = Some (GT () (λ '(), (latch (alloc_initialized)) : type)%I) →
     global_latch_wait ◁ᵥ global_latch_wait @ function_ptr type_of_latch_wait -∗
     global_test ◁ᵥ global_test @ function_ptr type_of_test -∗
     typed_function (impl_main2 global_initialized global_latch_wait global_test) type_of_main2.
